IRGraph.thy
@@ -9,17 +9,17 @@ begin
 
 (* This theory defines the main Graal data structure - an entire IR Graph. *)
 text_raw \<open>\Snip{graphdef}%\<close>
-type_synonym IRGraph = "(ID, IRNode) fmap"
+type_synonym IRGraph = "(ID fset \<times> (ID \<rightharpoonup> IRNode))"
 text_raw \<open>\EndSnip\<close>
 
 (* Get ALL the IDs in the graph. *)
-fun graph_nodes :: "IRGraph \<Rightarrow> ID set" where
-  "graph_nodes g = fset (fmdom g)"
+fun ids :: "IRGraph \<Rightarrow> ID set" where
+  "ids g = fset (fst g)"
 
 text_raw \<open>\Snip{helpers}%\<close>
 (* Look up a given ID in the graph and return the whole node. *)
 fun kind :: "IRGraph \<Rightarrow> ID \<Rightarrow> IRNode" where
-  "kind g nid = (case fmlookup g nid of 
+  "kind g nid = (case snd g nid of 
                  Some n \<Rightarrow> n | 
                  None \<Rightarrow> NoNode)"
 (* Get the inputs list of a given node ID. *)
@@ -27,10 +27,10 @@ fun inp :: "IRGraph \<Rightarrow> ID \<Rightarrow> ID list" where
   "inp g nid = inputs_of(kind g nid)"
 (* Gives a relation between node IDs - between a node and its input nodes. *)
 fun input_edges :: "IRGraph \<Rightarrow> ID rel" where
-  "input_edges g = (\<Union> i\<in>fset(fmdom g). {(i,j)|j. j \<in> fset(fset_of_list (inputs_of (kind g i)))})"
+  "input_edges g = (\<Union> i \<in> ids g. {(i,j)|j. j \<in> fset(fset_of_list (inputs_of (kind g i)))})"
 (* Find all the nodes in the graph that have nid as an input. *)
 fun usages :: "IRGraph \<Rightarrow> ID \<Rightarrow> ID set" where
-  "usages g nid = {j. j \<in> graph_nodes g \<and> (j,nid) \<in> input_edges g}"
+  "usages g nid = {j. j \<in> ids g \<and> (j,nid) \<in> input_edges g}"
 text_raw \<open>\EndSnip\<close>
 (* usages WAS:
   "usages g nid = fset (ffilter (\<lambda> nid' . nid \<in> set(inp g nid')) (fmdom g))"
@@ -41,7 +41,14 @@ text_raw \<open>\EndSnip\<close>
 fun succ :: "IRGraph \<Rightarrow> ID \<Rightarrow> ID list" where
   "succ g nid = successors_of(kind g nid)"
 
+fun is_empty :: "IRGraph \<Rightarrow> bool" where
+  "is_empty g = ((ids g = {}) \<and> (snd g = Map.empty))"
 
+definition empty_graph:: IRGraph where
+  "empty_graph = (fset_of_list [], Map.empty)"
+
+lemma empty_graph [simp]: "empty_graph = (fset_of_list [], Map.empty)"
+  by (rule empty_graph_def)
 
 
 (* First well-formedness predicate for IR graphs.
@@ -75,17 +82,18 @@ fun wff_graph :: "IRGraph \<Rightarrow> bool" where
 (* graph closure invariants *)
 text_raw \<open>\Snip{graphinvar}%\<close>
 fun has_good_inputs :: "ID \<Rightarrow> IRGraph \<Rightarrow> bool" where
-  "has_good_inputs n g = list_all (\<lambda>i. i |\<in>| fmdom g) (inputs_of (kind g n))"
+  "has_good_inputs n g = list_all (\<lambda>i. i \<in> ids g) (inputs_of (kind g n))"
 
 fun has_good_successors :: "ID \<Rightarrow> IRGraph \<Rightarrow> bool" where
-  "has_good_successors n g = list_all (\<lambda>i. i |\<in>| fmdom g) (successors_of (kind g n))"
+  "has_good_successors n g = list_all (\<lambda>i. i \<in> ids g) (successors_of (kind g n))"
 
 fun wff_graph :: "IRGraph \<Rightarrow> bool" where
   "wff_graph g = (
-    (g \<noteq> fmempty \<longrightarrow> is_StartNode (kind g 0)) \<and>
-    (\<forall> n. n |\<in>| fmdom g \<longrightarrow> has_good_inputs n g) \<and>
-    (\<forall> n. n |\<in>| fmdom g \<longrightarrow> has_good_successors n g) \<and>
-    (\<forall> n. n |\<in>| fmdom g \<longrightarrow> kind g n \<noteq> NoNode)
+    (\<not>(is_empty g) \<longrightarrow> is_StartNode (kind g 0)) \<and>
+    (\<forall> n. n \<in> ids g \<longrightarrow> has_good_inputs n g) \<and>
+    (\<forall> n. n \<in> ids g \<longrightarrow> has_good_successors n g) \<and>
+    (\<forall> n. n \<in> ids g \<longrightarrow> kind g n \<noteq> NoNode) \<and>
+    (\<forall> n. n \<in> ids g \<longrightarrow> n \<in> dom (snd g))
    )"
 text_raw \<open>\EndSnip\<close>
 (* TODO: add these other invariants?
@@ -99,16 +107,15 @@ text_raw \<open>\EndSnip\<close>
 
 lemma wff_kind [simp]:
   assumes "wff_graph g"
-  assumes "n |\<in>| fmdom g"
+  assumes "n \<in> ids g"
   shows "kind g n \<noteq> NoNode"
   using assms by auto
 
+fun irgraph :: "(ID \<times> IRNode) list \<Rightarrow> IRGraph" where
+  "irgraph g = (fset_of_list (map fst g), map_of g)"
 
-definition empty_graph:: IRGraph where
-  "empty_graph = fmempty"
-
-lemma empty_graph [simp]: "empty_graph = fmempty"
-  by (rule empty_graph_def)
+fun add_node :: "nat \<Rightarrow> IRNode \<Rightarrow> IRGraph \<Rightarrow> IRGraph" where
+  "add_node nid node g = ((fset_of_list [nid]) |\<union>| (fst g), (snd g)(nid \<mapsto> node))"
 
 (* Example 1: empty graph (just a start node) *)
 lemma wff_empty: "wff_graph empty_graph"
@@ -126,7 +133,7 @@ lemma wff_empty: "wff_graph empty_graph"
       [5 Return]
 *)
 definition eg2_sq :: IRGraph where
-  "eg2_sq = fmap_of_list [
+  "eg2_sq = irgraph [
     (0, StartNode None 5),
     (1, ParameterNode 0),
     (4, MulNode 1 1),
